prophecy/ProphecyRA.v
@@ -2,8 +2,6 @@ Require Import CRIS.
 Require Import ProphecyHeader Ensembles.
 From iris.algebra Require Import auth excl functions.
 
-Set Implicit Arguments.
-
 Definition ProphInst : Type :=
   { P : Prophecy.t & (P.(Prophecy.Pro) * list P.(Prophecy.Obs))%type }.
 Canonical Structure ProphInstO := leibnizO ProphInst.
@@ -24,7 +22,7 @@ Global Instance subG_prophG `{!crisG Γ Σ α β τ _I _S} : subG prophΓ Γ →
 Proof. solve_inG. Defined.
 
 Section ProphecyRA.
-  Context `{!crisG Γ Σ α β τ _I _S, _PROPH: !prophGS}.
+  Context `{!crisG Γ Σ α β τ _I _S, !prophGS}.
 
   Definition dummy_proph : Prophecy.t :=
     {| Prophecy.Pro := ();
@@ -42,6 +40,10 @@ Section ProphecyRA.
     discrete_fun_singleton id (◯E v).
   Definition has_proph (id : Prophecy.ID) (v : ProphInst) : iProp Σ :=
     own proph_name (has_proph_r id v).
+  Definition syn_has_proph {n} (id : Prophecy.ID) (v : ProphInst) : GTerm.t n :=
+    sown proph_name (has_proph_r id v).
+  Global Instance has_proph_red {n} id v : SLRed n (syn_has_proph id v) (has_proph id v).
+  Proof. solve_sl_red. Qed.
 
   Definition has_proph_auth_r (P : Prophecy.ID → Prop) (map : Prophecy.ID -> ProphInst) : ProphRA :=
     λ id,
@@ -117,5 +119,5 @@ Proof.
     { apply auth_both_valid_discrete; split; ss. }
     { rewrite right_id auth_auth_valid //. }
   }
-  by iExists (Build_prophGS _ γp γi); rewrite own_op; iFrame.
+  by iExists (Build_prophGS _ _ _ _ _ _ _ _ _ γp γi); rewrite own_op; iFrame.
 Qed.
