prophecy/ProphecyFacts.v
@@ -1,4 +1,5 @@
-Require Export CRIS CallFilter ProphecyIAproof.
+Require Export CRIS CallFilter ProphecyIAproof HelpingFacts.
+Require Export SchI MemI MemA MemIAproof.
 From stdpp Require Import base list.
 
 Lemma CFilter_real_mod `{Σ : GRA} (md : Mod.t) (msk : gset string) :
@@ -90,5 +91,124 @@ Section prophecy.
 
     rewrite Mod.add_comm.
     eapply ctxr_refines, ctxr_cond_strengthen; iIntros "[$ [$ $]]".
+  Qed.
+
+  Lemma helping_prophecy_refines
+      `{!memGS}
+      (mds mdt ctx : Mod.t) (mdp mdm : string → Mod.t) csl genv sp_mem sp_help
+      {jobID retID} (jobs : jobID → itree crisE retID) :
+    let fns mn := ProphecyName.exports mn ∪ Helping.exports mn in
+    (∀ mn,
+      ctx_refines
+        (mdp mn ★ ProphecyI.t mn, emp%I) (CFilter.filter (fns mn) mdt ★ ProphecyI.t mn, emp%I)) →
+    (∀ mn,
+      ctx_refines
+        (mdm mn ★ HelpingOn.t mn jobs sp_help ★ MemA.t sp_mem ★ ProphecyA.t mn ∅, emp%I)
+        (mdp mn ★ HelpingDummy.t mn ★ MemA.t sp_mem ★ ProphecyA.t mn ∅, emp%I)) →
+    (∀ mn, ctx_refines (mds, emp%I) (mdm mn ★ HelpingOff.t mn jobs sp_help, emp%I)) →
+    real_mod ctx →
+    (∀ mn, real_mod (mdp mn)) →
+    refines
+      (mds ★ MemA.t sp_mem ★ SchI.t ★ ctx, MemA.init_cond csl genv ∗ ProphecyA.initial_cond)%I
+      (mdt ★ MemI.t csl genv ★ SchI.t ★ ctx, emp%I).
+  Proof.
+    intros fns Hproph_insert Hmain Herase Hctx_real Hmdp_real.
+    assert (Hadd_wf : ∀ mn, Mod.wf (ProphecyI.t mn ★ HelpingDummy.t mn)).
+    { i; econs; [mod_tac|prove_nodup]. }
+    set (l := maxlen
+      (elements (set_omap (λ a, match a with | fid fn => Some fn | _ => None end) (dom (Mod.fnsems (SchI.t ★ ctx ★ MemA.t sp_mem ★ mds))) : gset string) ++
+       elements (set_omap (λ a, match a with | fid fn => Some fn | _ => None end) (dom (Mod.fnsems (mdt ★ MemI.t csl genv ★ SchI.t ★ ctx))) : gset string) ++
+       Mod.scopes (mdt ★ MemI.t csl genv ★ SchI.t ★ ctx) ++
+      Mod.scopes mdt ++ Mod.scopes ctx ++ Mod.scopes mds)).
+    set (mn := mname_long (S l)).
+    assert (mn ∉ Mod.scopes (mdt ★ MemI.t csl genv ★ SchI.t ★ ctx)) as Hmn.
+    { intros Hcontra%elem_of_maxlen; subst mn l.
+      rewrite !mname_long_length ?maxlen_union in Hcontra; lia.
+    }
+    etrans; cycle 1.
+    { eapply ctxr_refines, CFilter.intro_filter with (fns := fns mn). }
+    etrans; cycle 1.
+    { eapply CFilter.intro_module with (mc := ProphecyI.t mn ★ HelpingDummy.t mn).
+      { apply Hadd_wf. }
+      { revert Hmn; generalize mn; clear dependent mn. intros ? ?. set_solver+Hmn. }
+      { intros i Hi1 Hi2; rewrite -elem_of_elements in Hi1; eapply elem_of_maxlen in Hi1.
+        subst fns; set_unfold in Hi2; des; subst mn l; subst;
+          rewrite string_length_app ?mname_long_length ?maxlen_union in Hi1; lia.
+      }
+      { clear. generalize mn; clear dependent mn l; subst fns; intros ?.
+        rewrite Mod.dom_fnsems_add set_omap_union; set_solver. }
+      { clear. generalize mn; clear dependent mn l; intros ?.
+        rewrite Mod.dom_fnsems_add. set_solver+. }
+    }
+    do 2 rewrite CFilter.filter_app.
+    etrans; cycle 1.
+    { eapply ctxr_refines.
+      ctxr_rotate. do 2 ctxr_drop. ctxr_rotate. ctxr_drop.
+      eapply (Hproph_insert).
+    }
+    etrans; cycle 1.
+    { rewrite ?assoc.
+      eapply ProphIA.adequacy_refines; eauto.
+      rewrite -!assoc CFilter.filter_app.
+      repeat eapply real_mod_add; eauto using CFilter_real_mod.
+      { apply CFilter_real_mod. rewrite /real_mod.
+        clear dependent mn l.
+        let real_tac :=
+          (split; ss; intros ??; destruct excluded_middle_informative; ss) in
+        mod_tac real_tac.
+       }
+      { apply CFilter_real_mod. rewrite /real_mod.
+        clear.
+        let real_tac :=
+          (split; ss; intros ??; destruct excluded_middle_informative; ss) in
+        mod_tac real_tac.
+      }
+      { rewrite /real_mod.
+        clear. generalize mn; clear dependent mn l; intros ?.
+        let real_tac :=
+          (split; ss; intros ??; destruct excluded_middle_informative; ss) in
+        mod_tac real_tac.
+      }
+    }
+    etrans; cycle 1.
+    { eapply ctxr_refines. ctxr_rotate. do 4 ctxr_drop.
+      clear. generalize mn; clear dependent mn l; intros ?.
+      eapply main_adequacy, MemIA.sim; set_solver.
+    }
+    etrans; cycle 1.
+    { eapply ctxr_refines.
+      ctxr_drop. ctxr_swap. do 2 ctxr_rotate. ctxr_swap. do 2 ctxr_rotate.
+      eapply Hmain.
+    }
+    rewrite CFilter.filter_app.
+    etrans; cycle 1.
+    { eapply ctxr_refines. ctxr_rotate. ctxr_drop. ctxr_drop. ctxr_swap. ctxr_drop.
+      ctxr_swap. ctxr_drop.
+      eapply helping_onoff_correct; eauto.
+      clear. generalize mn; clear dependent mn l; intros ?.
+      set_solver.
+    }
+    etrans; cycle 1.
+    { eapply ctxr_refines. ctxr_drop. do 2 (ctxr_swap; ctxr_drop). rewrite /mod_src.
+      do 2 ctxr_rotate. ctxr_drop. eapply Herase.
+    }
+    etrans; cycle 1.
+    { eapply ctxr_refines. do 2 ctxr_drop. ctxr_rotate. do 2 ctxr_drop. eapply elim_module. }
+    etrans; cycle 1.
+    { eapply ctxr_refines. ctxr_rotate. ctxr_drop. ctxr_swap; ctxr_drop. rewrite left_id.
+      erewrite <-!CFilter.filter_app. refl.
+    }
+    etrans; cycle 1.
+    { eapply ctxr_refines. do 2 ctxr_rotate. ctxr_drop. eapply CFilter.intro_filter. }
+    erewrite <-!CFilter.filter_app.
+    etrans; cycle 1.
+    { eapply CFilter.elim_filter.
+      rewrite -assoc.
+      intros i Hi1 Hi2; rewrite -elem_of_elements in Hi1; eapply elem_of_maxlen in Hi1.
+      subst fns; set_unfold in Hi2; des; subst mn l; subst;
+        rewrite string_length_app ?mname_long_length ?maxlen_union in Hi1; lia.
+    }
+    eapply ctxr_refines.
+    ctxr_norm. do 3 ctxr_rotate. ctxr_drop. do 2 ctxr_rotate. ctxr_drop. refl.
   Qed.
 End prophecy.
